absorbs <-> does not absurd

sha3/proof/LeakyAbsorb.ec
@@ -1,17 +1,16 @@
 (* -------------------------------------------------------------------- *)
-require import Option Pair Int Real List FSet NewFMap.
-require (*--*) LazyRP RndOrcl.
+require import Option Pair Int Real Distr List FSet NewFMap.
+require (*--*) LazyRP RndOrcl. 
 (*---*) import Dprod.
 
 (* -------------------------------------------------------------------- *)
-op r : { int | 0 < r } as gt0_r.
-op c : { int | 0 < c } as gt0_c.
 
 type block.    (* = {0,1}^r *)
 type capacity. (* = {0,1}^c *)
 
 op cdist : capacity distr.
 op bdist : block distr.
+axiom bdist_ll : weight bdist = 1%r.
 
 (* isomorphic to the {0,1}^? uniform distributions *)
 
@@ -41,19 +40,32 @@ module type WeirdIRO_ = {
 
 op valid_query : block list -> int -> bool.
 op valid_queries : (block list) fset.
-axiom valid_queryP : forall m n, valid_query m n => mem valid_queries (m ++ map (fun x => b0) (iota_ 0 n)).
+axiom valid_queryP     : forall m n, valid_query m n => forall k, 0 <= k <= n => mem valid_queries (m ++ map (fun x => b0) (iota_ 0 k)).
+axiom valid_query_take : forall m n, valid_query m n => forall i, 0 <= i <= size m => mem valid_queries (take i m).
+axiom valid_query_take1 : 
+  forall m n, valid_query m n => forall i, 0 <= i <= size m => valid_query (take i m) 1.
+axiom valid_query_size : forall m n, valid_query m n => 1 <= size m.
 
-module IdealFunctionalityThatDoesNotAbsorb = {
+module type RO = {
+  proc init () : unit
+  proc f(_:block list) : block 
+}.
+
+module Ro = {
   var h : (block list,block) fmap
 
   proc init() = { h = map0; }
 
-  proc core(m : block list) = {
-    if (!mem (dom h) m) {
-      h.[m] <$ bdist;
-    }
+  proc f(m : block list) = {
+    var r;
+    r <$ bdist;
+    if (!mem (dom h) m) h.[m] <- r ;
     return oget h.[m];
   }
+}.
+
+module GenIdealFunctionalityThatDoesNotAbsorb(Ro:RO) = {
+  proc init = Ro.init
 
   proc f(m : block list, n : int) = {
     var i <- 1;
@@ -64,40 +76,44 @@ module IdealFunctionalityThatDoesNotAbsorb = {
     if (valid_query m n) {
       while (j <= size m) {
         z <- rcons z b;
-        b <@ core(take j m);
+        b <@ Ro.f(take j m);
         j <- j + 1;
       }
       while (i < n) {
         z <- rcons z b;
         m <- rcons m b0;
-        b <@ core(m);
-        j <- j + 1;
+        b <@ Ro.f(m);
+        i <- i + 1;
       }
     }
     return z;
   }
 }.
 
-module IdealFunctionalityThatAbsorbs = {
-  proc init = IdealFunctionalityThatDoesNotAbsorb.init
+module IdealFunctionalityThatDoesNotAbsorb = GenIdealFunctionalityThatDoesNotAbsorb(Ro).
+
+module GenIdealFunctionalityThatAbsorbs(Ro:RO) = {
+  proc init = Ro.init 
 
   proc f(m : block list, n : int) = {
-    var j <- 1;
+    var i <- 1;
     var z <- [];
     var b;
 
     if (valid_query m n) {
-      b <@ IdealFunctionalityThatDoesNotAbsorb.core(m);
-      while (j < n) {
+      b <@ Ro.f(m);
+      while (i < n) {
         z <- rcons z b;
         m <- rcons m b0;
-        b <@ IdealFunctionalityThatDoesNotAbsorb.core(m);
-        j <- j + 1;
+        b <@ Ro.f(m);
+        i<- i + 1;
       }
     }
     return z;
   }
 }.
+
+module IdealFunctionalityThatAbsorbs = GenIdealFunctionalityThatAbsorbs(Ro).
 
 (* -------------------------------------------------------------------- *)
 module type CONSTRUCTION(P : RP) = {
@@ -106,7 +122,7 @@ module type CONSTRUCTION(P : RP) = {
   proc f(bp : block list, n : int) : block list
 }.
 
-module type SIMULATOR(F : WeirdIRO) = {
+module type SIMULATOR(F : WeirdIRO_) = {
   proc init() : unit
 
   proc f(_ : block * capacity) : block * capacity
@@ -205,17 +221,18 @@ section PROOF.
   (* From Absord to do Not *)
   module MkD (D:DISTINGUISHER, F:WeirdIRO_, P:RP_) = D(MkF(F),P).
 
-  module MkFdoNot (F:WeirdIRO) = {
-    proc init = F.init
+  module MkFdoNot1 (F:WeirdIRO_) = {
     proc f(m:block list, n:int) : block list = {
       var i, r, tl, b;
       r <- [];
       if (valid_query m n) {
-        i <- 0;
-        while (i < size m - 1) {
+        i <- 1;
+        b <- [b0]; 
+        while (i <= size m) {
+          r <- r ++ b;
           b <- F.f(take i m, 1);
           i <- i + 1;
-          r <- r ++ b;
+
         }
         tl <- F.f(m,n);
         r  <- r ++ tl;
@@ -224,16 +241,127 @@ section PROOF.
     }
   }.
 
+  module MkFdoNot (F:WeirdIRO) = {
+    proc init = F.init
+    proc f = MkFdoNot1(F).f
+  }.
+
   module MkS(S:SIMULATOR, F:WeirdIRO) = S(MkFdoNot(F)).
 
-  local clone 
+  local clone RndOrcl as RndOrcl0 with 
+    type from <- block list, 
+    type to   <- block.
+  
+  local clone RndOrcl0.RestrIdeal as RI with
+    op sample <- fun (bl:block list) => bdist,
+    op test   <- (mem valid_queries),
+    op univ   <- valid_queries,
+    op dfl    <- b0
+    proof *.
+  realize sample_ll. by move=> _;apply bdist_ll. qed.
+  realize testP. by []. qed.
+  import RI.
+
+  local module E1 (Ro:RO) = {
+    module F = { 
+      proc f = GenIdealFunctionalityThatDoesNotAbsorb(Ro).f
+    }
+    module P = S(F)
+    proc distinguish () : bool = {
+      var b;
+      P.init();
+      b <@  MkD(D, F, P).distinguish();
+      return b;
+    }
+  }.
+
+  local module E2 (Ro:RO) = {
+    module F = { 
+      proc f = GenIdealFunctionalityThatAbsorbs(Ro).f
+    }
+    module P = S(MkFdoNot1(F)) 
+    proc distinguish () : bool = {
+      var b;
+      P.init();
+      b <@  D(F, P).distinguish();
+      return b;
+    }
+  }.
+
+  local equiv f_f : 
+    GenIdealFunctionalityThatDoesNotAbsorb(Ro).f ~ E1(Restr(RO)).F.f : 
+    ={m, n} /\ Ro.h{1} = RO.m{2} ==> ={res} /\ Ro.h{1} = RO.m{2}.
+  proof.
+    proc;sp;if => //.
+    inline{2} Restr(RO).f.
+    while (={z,i,n,b,m} /\ Ro.h{1} = RO.m{2} /\ 
+              (forall k, 0 <= k <= n - i => mem valid_queries (m ++ map (fun x => b0) (iota_ 0 k))){2}).
+    + rcondt{2} 5=> //. 
+      + auto;progress; rewrite - cats1;cut := H 1 _; [by smt| by rewrite iota1].  
+      auto; call (_:Ro.h{1} = RO.m{2});[by sim | auto;progress].
+      cut := H (k+1) _;1:by smt.
+      rewrite iotaS //= -cats1 -catA /= (_:  map (fun (x : int) => b0) (iota_ 1 k) = map (fun (x : int) => b0) (iota_ 0 k)) //.
+      by rewrite (iota_addl 1 0 k) -map_comp;apply eq_map.
+    while (={z,j,n,b,m} /\ Ro.h{1} = RO.m{2} /\ valid_query m{1} n{1} /\ 0 <= j{1}).
+    + rcondt{2} 4=> //. 
+      + auto;progress;apply (valid_query_take _ _ H)=> //.
+      auto; call (_:Ro.h{1} = RO.m{2});[by sim | auto;progress;smt].
+    skip;progress;apply (valid_queryP _ _ H2);smt.
+  qed.
+
+  local equiv f_f_a :  GenIdealFunctionalityThatAbsorbs(Ro).f ~ E2(Restr(RO)).F.f : ={m,n} /\ Ro.h{1} = RO.m{2} ==> ={res} /\ Ro.h{1} = RO.m{2}. 
+  proof.
+    proc; sp;if=> //;inline{2} Restr(RO).f;sp.
+    rcondt{2} 1=> //.
+    + auto;progress;cut := valid_query_take _ _ H (size m{hr}).
+      rewrite take_size=> HH;apply HH;smt.
+    while (={z,i,n,b,m} /\ Ro.h{1} = RO.m{2} /\ 
+                (forall k, 0 <= k <= n - i => mem valid_queries (m ++ map (fun x => b0) (iota_ 0 k))){2}).
+    + rcondt{2} 5=> //. 
+      + auto;progress; rewrite -cats1;cut := H 1 _; [by smt| by rewrite iota1].  
+      auto; call (_:Ro.h{1} = RO.m{2});[by sim | auto;progress].
+      cut := H (k+1) _;1:by smt.
+      rewrite iotaS //= -cats1 -catA /= (_:  map (fun (x : int) => b0) (iota_ 1 k) = map (fun (x : int) => b0) (iota_ 0 k)) //.
+      by rewrite (iota_addl 1 0 k) -map_comp;apply eq_map.
+    wp;call (_:Ro.h{1} = RO.m{2});[by sim | auto;progress]. 
+    apply (valid_queryP _ _ H);smt.
+  qed.
+
+  local equiv f_f' : 
+    MkFdoNot(GenIdealFunctionalityThatAbsorbs(Ro)).f ~ MkFdoNot1(E2(Restr(RO)).F).f :
+    ={m, n} /\ Ro.h{1} = RO.m{2} ==>
+    ={res} /\ Ro.h{1} = RO.m{2}.
+  proof.
+    proc;sp;if => //;wp.
+    call f_f_a. 
+    while (={i,m,r,b} /\ Ro.h{1} = RO.m{2} /\ valid_query m{1} n{1} /\ 0 <= i{1});last by auto.
+    wp; call f_f_a;auto;progress;smt.
+  qed.
+ 
+  local equiv f_dN : E1(ERO).F.f ~ MkFdoNot1(E2(ERO).F).f : ={m, n} /\ ={RO.m} ==> ={res, RO.m}.
+  proof.
+    proc;sp;if=> //;sp.
+    inline {2} E2(ERO).F.f.
+    rcondt{2} 6;auto; 1: by conseq (_: _ ==> true).
+    while (={RO.m} /\ z{1} = r{2} ++ z0{2} /\ i{1} = i1{2} /\ n{1} = n1{2} /\ b{1} = b1{2} /\
+           m{1} = m1{2}).
+    + inline *;auto;progress;smt. 
+    inline ERO.f;auto.
+    while (={RO.m,m,n} /\ z{1} = r{2} /\ b{2} = [b{1}] /\ valid_query m{1} n{1} /\ 
+           j{1} = i{2} /\ 0 <= i{2} /\
+           (1 < j => b =  mem valid_queries (take j m) ? oget RO.m.[x]  : Self.b0){1}).
+    + rcondt{2} 6;1:by auto;progress;smt. 
+      rcondf{2} 8;1:by auto.
+      auto;progress;smt.
+    auto;progress;smt. 
+  qed.
 
   lemma conclusion &m:
     `| Pr[Experiment(SpongeThatDoesNotAbsorb(Perm), Perm, MkD(D)).main() @ &m : res]
         - Pr[Experiment(IdealFunctionalityThatDoesNotAbsorb, 
              S(IdealFunctionalityThatDoesNotAbsorb), MkD(D)).main() @ &m : res] | = 
-    `|Pr[Experiment(SpongeThatAbsorbs(Perm),Perm,D).main() @ &m : res] -
-      -Pr[Experiment(IdealFunctionalityThatAbsorbs, MkS(S,IdealFunctionalityThatAbsorbs), D).main() @ &m : res]|.
+    `|Pr[Experiment(SpongeThatAbsorbs(Perm),Perm,D).main() @ &m : res] 
+      - Pr[Experiment(IdealFunctionalityThatAbsorbs, MkS(S,IdealFunctionalityThatAbsorbs), D).main() @ &m : res]|.
   proof.
     congr;congr.
     + byequiv (_: ={glob D} ==> _) => //;proc;inline *.
@@ -245,31 +373,44 @@ section PROOF.
       while (={glob Perm, p, sa,sc} /\ (size z = size m - size p){1}).
       + wp;call (_ : ={glob Perm});[by sim|auto;progress [-split];smt].
       by auto;progress [-split];smt. 
-    +      
-      auto. 
-
-smt. smt.
-search drop.          
-        
-sim.
-
-
-
-
-op eps : real.
-
-axiom core:
-  exists (S <: SIMULATOR),
-    forall (D <: DISTINGUISHER) &m,
-      `|  Pr[Experiment(SpongeThatDoesNotAbsorb(Perm), Perm, D).main() @ &m : res]
-        - Pr[Experiment(IdealFunctionalityThatDoesNotAbsorb, S(IdealFunctionalityThatDoesNotAbsorb), D).main() @ &m : res]|
-       < eps.
-
-lemma top:
-  exists eps',
-    exists (S <: SIMULATOR),
-      forall (D <: DISTINGUISHER) &m,
-        `|  Pr[Experiment(SpongeThatAbsorbs(Perm), Perm, D).main() @ &m : res]
-          - Pr[Experiment(IdealFunctionalityThatAbsorbs, S(IdealFunctionalityThatAbsorbs), D).main() @ &m : res]|
-         < eps'.
-proof. admit. (** FILL ME IN **) qed.
+    cut -> : Pr[Experiment(IdealFunctionalityThatDoesNotAbsorb, S(IdealFunctionalityThatDoesNotAbsorb), MkD(D)).main () @ &m : res] =
+               Pr[RndOrcl0.IND(Restr(RO), E1).main() @ &m : res].
+    + byequiv=> //. (* PY: BUG printer res *)
+      proc;inline{2} E1(Restr(RO)).distinguish;auto.
+      call (_: ={glob S} /\ Ro.h{1} = RO.m{2}). 
+      + by proc (Ro.h{1} = RO.m{2}) => //;apply f_f.
+      + by proc (Ro.h{1} = RO.m{2}) => //;apply f_f.
+      + by proc;sp;if=> //;wp;call f_f.
+      by inline *; call (_: Ro.h{1} = RO.m{2});auto;apply f_f.
+    cut -> : Pr[Experiment(IdealFunctionalityThatAbsorbs, MkS(S, IdealFunctionalityThatAbsorbs), D).main() @ &m : res] = 
+               Pr[RndOrcl0.IND(Restr(RO), E2).main() @ &m : res].
+    + byequiv=> //. 
+      proc;inline{2} E2(Restr(RO)).distinguish;auto.
+      call (_: ={glob S} /\ Ro.h{1} = RO.m{2}). 
+      + proc (Ro.h{1} = RO.m{2}) => //; apply f_f'.
+      + by proc (Ro.h{1} = RO.m{2}) => //;apply f_f'.
+      + conseq f_f_a => //. 
+      by inline *;call (_:Ro.h{1} = RO.m{2});[apply f_f'|auto].
+    cut -> : Pr[RndOrcl0.IND(Restr(RO), E1).main() @ &m : res] = 
+             Pr[RndOrcl0.IND(ERO, E1).main() @ &m : res].
+    + byequiv (Eager E1)=> //.
+    cut -> : Pr[RndOrcl0.IND(Restr(RO), E2).main() @ &m : res] = 
+             Pr[RndOrcl0.IND(ERO, E2).main() @ &m : res].
+    + byequiv (Eager E2)=> //.
+    byequiv=> //.
+    proc; inline *;wp.
+    call (_: ={RO.m, glob S}).
+    + by proc (={RO.m})=> //;apply f_dN.
+    + by proc (={RO.m})=> //;apply f_dN.
+    + proc;sp;if => //.
+      inline{1} E1(ERO).F.f;sp;rcondt{1} 1; 1:by auto.
+      wp;while (={RO.m,i,b} /\ n0{1} = n{2} /\ m0{1} = m{2} /\ z{1} = take (size m{1}) z{1} ++ z{2} /\ (size m <= size z){1}).
+      + inline *;auto;progress [-split]; smt. 
+      inline *;splitwhile{1} 1 : (j < size m0).
+      wp;seq 1 0 : (={i,RO.m, m, glob S} /\ n0{1} = n{2} /\ m0{1} = m{2} /\ size m0{1} - 1 = size z{1} /\ size m0{1} = j{1} /\ z{2} = []).
+      while{1} (size z{1} = j{1} - 1 /\ j{1} <= size m0{1}) ((size m0 - j){1});auto;progress [-split]; smt. 
+      rcondt{1} 1;1:by auto. 
+      rcondf{1} 5;auto;progress[-split];smt. 
+    call (_: ={RO.m})=> //;1:by apply f_dN.
+    sim : (={glob S, glob D, RO.m})=> //. 
+  qed.
